Test/og/treiber-stack.bpl
@@ -1,48 +1,39 @@
 type Node;
 type lmap;
-function dom(lmap): [Node]bool;
+function {:linear "Node"} dom(lmap): [Node]bool;
 function map(lmap): [Node]Node;
 
-function {:builtin "MapConst"} MapConst(bool) : [Node]bool;
-function {:builtin "MapOr"} MapOr([Node]bool, [Node]bool) : [Node]bool;
+procedure {:yields} Load(i:Node) returns(v:Node);
+requires dom(stack)[i];
+ensures {:atomic 0} v == map(stack)[i];
 
-procedure Load(i:Node) returns(v:Node);
-  requires dom(stack)[i];
-  ensures  v == map(stack)[i];
+procedure {:yields} Store({:linear "Node"} l_in:lmap, i:Node, v:Node) returns({:linear "Node"} l_out:lmap);
+requires dom(l_in)[i];
+ensures {:atomic 0} dom(l_out) == dom(l_in) && map(l_out) == map(l_in)[i := v];
 
-procedure Store({:linear "Node"} l_in:lmap, i:Node, v:Node) returns({:linear "Node"} l_out:lmap);
-  requires dom(l_in)[i];
-  ensures  dom(l_out) == dom(l_in);
-  ensures  map(l_out) == map(l_in)[i := v];
+procedure {:yields} TransferToStack(oldVal: Node, newVal: Node, {:linear "Node"} l_in:lmap) returns (r: bool, {:linear "Node"} l_out:lmap);
+requires dom(l_in)[newVal];
+modifies stack, TOP;
+ensures {:atomic 0} if oldVal == old(TOP)
+		    then newVal == TOP && dom(stack) == dom(old(stack))[newVal := true] && map(stack) == map(old(stack))[newVal := map(l_in)[newVal]]
+                    else TOP == old(TOP) && stack == old(stack) && l_out == l_in;
 
-procedure TransferIn({:linear "Node"} l1_in:lmap, d:Node);
-  requires dom(l1_in)[d];
-  modifies stack;
-  ensures  dom(stack) == dom(old(stack))[d := true];
-  ensures  map(stack) == map(old(stack))[d := map(l1_in)[d]];
+procedure {:yields} TransferFromStack(oldVal: Node, newVal: Node) returns (r: bool, {:linear "Node"} l_out:lmap);
+requires dom(stack)[oldVal];
+modifies stack, TOP;
+ensures {:atomic 0} if oldVal == old(TOP)
+		    then dom(stack) == dom(old(stack))[oldVal := false] && map(stack) == map(old(stack)) && dom(l_out)[oldVal] && map(l_out)[oldVal] == map(old(stack))[oldVal]
+		    else TOP == old(TOP) && stack == old(stack);
 
-procedure TransferOut(d:Node);
-  requires dom(stack)[d];
-  modifies stack;
-  ensures  dom(stack) == dom(old(stack))[d := false];
-  ensures  map(stack) == map(old(stack));
-
-procedure New() returns ({:linear "Node"} l: lmap, d: Node);
+procedure Alloc() returns (d: Node, {:linear "Node"} l: lmap);
 ensures dom(l)[d];
+
+procedure Free(d: Node, {:linear "Node"} l: lmap);
 
 const unique null: Node;
 
-var TOP: Node;
-var {:linear "Node"} stack: lmap;
-
-procedure {:yields} CAS(oldVal: Node, newVal: Node)
-returns (r: bool)
-{
-  r := (TOP == oldVal);
-  if (r) {
-    TOP := newVal;
-  }
-}
+var {:qed} TOP: Node;
+var {:qed} {:linear "Node"} stack: lmap;
 
 procedure {:yields} push()
 {
@@ -50,15 +41,14 @@ procedure {:yields} push()
   var g: bool;
   var {:linear "Node"} x_lmap: lmap;
 
-  call x_lmap, x := New();
+  call x, x_lmap := Alloc();
 
   while(true)
   {
     t := TOP;		
     call x_lmap := Store(x_lmap, x, t);
-    call g := CAS(t, x); 
+    call g, x_lmap := TransferToStack(t, x, x_lmap); 
     if (g) { 
-      call TransferIn(x_lmap, x);
       break; 
     }
   }
@@ -68,6 +58,7 @@ procedure {:yields} pop()
 {
   var t, x: Node;
   var g: bool;
+  var {:linear "Node"} t_lmap: lmap;
 
   while(true)
   {
@@ -77,9 +68,9 @@ procedure {:yields} pop()
       return;
     }
     call x := Load(t);
-    call g := CAS(t, x); 
+    call g, t_lmap := TransferFromStack(t, x); 
     if (g) { 
-      call TransferOut(t);
+      call Free(t, t_lmap);
       break; 
     }
   }
